add induction notes

Notes4/Induction.lean
@@ -1,3 +1,93 @@
+import Mathlib.Data.Nat.Basic
 import Mathlib.Tactic.Cases
+import Notes4.IndTypes
+/- 
+Induction with Inductive Types
 
+Let's see a bit how how induction is called inductive types. 
+For each inductive type, recursors are automatically instantiated. 
+-/
 
+#check Nat.rec
+#check List.rec
+
+example (a b c: ℕ) : exp (a*b) c = (exp a c) * exp b c := by 
+  apply @Nat.rec (fun c => exp (a*b) c = ((exp a c) * exp b c))
+  · simp [exp]
+  · intro n ih 
+    simp [exp]
+    rw [ih]
+    ac_rfl
+
+/-
+
+Using the recusors directly is not as ergnomic as some built in tactics 
+of which there are few.
+
+First, we have already seen that `match` can be used to argue via 
+induction. 
+
+Let's prove that our exponentiation function on ℕ is multiplicative in 
+the base. 
+-/
+
+theorem mul_of_mul_base_exp (a b c : ℕ) : exp (a*b) c = (exp a c) * exp b c := by 
+  match c with 
+  | 0 => simp only [exp] 
+  | c+1 => 
+    simp only [exp,Nat.add] 
+    rw [mul_of_mul_base_exp a b c]
+    ac_rfl
+
+/-
+
+In `mul_of_mul_base_exp`, we used induction at the step `rw [mul_of_mul_base_exp a b c]` 
+since this presumes a proof of `mul_of_mul_base_exp a b c`.
+
+Consider the following version using an anonymous `example`. 
+
+example (a b c: ℕ) : exp (a*b) c = (exp a c) * exp b c := by 
+  match c with 
+  | 0 => simp only [exp] 
+  | c+1 => 
+    simp only [exp,Nat.add] 
+    -- how do we call the inductive step without a name?
+    sorry 
+
+In this case, we can use `induction` or `induction'`. 
+
+-/
+
+variable {α : Type} 
+
+open List
+
+def iterateAppend : ℕ → List α → List α
+  | 0, _ => [] 
+  | n+1, l => l ++ iterateAppend n l
+
+-- Using `induction` 
+example (n : ℕ) (l : List α) : n*(l.length) = (iterateAppend n l).length := by 
+  induction n with 
+  | zero => 
+    simp only [iterateAppend,length]
+    rw [Nat.zero_mul]
+  | succ n' ih => 
+    simp [iterateAppend,length]
+    rw [Nat.succ_mul]
+    rw [ih]
+    ac_rfl 
+
+-- Using `induction'`
+example (n : ℕ) (l : List α) : n*(l.length) = (iterateAppend n l).length := by 
+  induction' n with m indhyp 
+  · simp only [iterateAppend,length]
+    rw [Nat.zero_mul] 
+  · simp [iterateAppend,length]
+    rw [Nat.succ_mul]
+    rw [indhyp]
+    ac_rfl 
+
+example (n m : ℕ) : n*m = m*n := sorry 
+
+example (a n m : ℕ) : a*(m + n) = a*m + a*n := sorry 
